Modify Incr*.v to exploit atomicity

incr/IncrAll.v
@@ -1,6 +1,6 @@
 Require Import CRIS Cancel.
 Require Import MemI MemA MemIAproof ImpPrelude.
-Require Import IncrMainHeader IncrMainI IncrMainA IncrMainIAproof.
+Require Import IncrHeader IncrI IncrA IncrIAproof.
 Require Import SchHeader SchI SchA SchIAproof SchTactics.
 
 Module IncrAll.
@@ -10,7 +10,7 @@ Module IncrAll.
   Local Definition csl : string → bool := λ _, false.
   Local Definition genv : GEnv.t := GEnv.unit.
 
-  Local Instance Γ : HRA := ##[invΓ; memΓ; SchAΓ; IncrMainAΓ].
+  Local Instance Γ : HRA := ##[invΓ; memΓ; SchAΓ; IncrAΓ].
   Local Instance Σ : GRA := ##[invΣ; SchAΣ; Γ].
 
   Definition IRΓ : Γ :=
@@ -28,33 +28,33 @@ Module IncrAll.
 
   (* source module *)
   Local Definition spc_user_s : string → option fspec :=
-    to_spc (IncrMainAS.spc u ++ MemA.spc).
+    to_spc (IncrAS.spc u ++ MemA.spc).
   Local Definition smod_src : SMod.t :=
-    (IncrMainA.Mod u) ☆ (MemA.Mod) ☆ (SchA.Mod u spc_user_s ☆ SchA_link.Mod u).
+    (IncrA.Mod u) ☆ (MemA.Mod) ☆ (SchA.Mod u spc_user_s ☆ SchA_link.Mod u).
   Local Definition spc_s : string → option fspec := spc_from smod_src.
 
   Local Definition smod_cancel : HMod.t := SModCancel.to_hmod smod_src.
   Local Definition mod_src : HMod.t := SMod.to_hmod (wsim_ginv u ⊤) spc_s smod_src.
-  Local Definition mod_tgt : HMod.t := IncrMainI.t ★ (MemI.t csl genv) ★ (SchI.t).
+  Local Definition mod_tgt : HMod.t := (IncrI.t ★ FaaI.t) ★ (MemI.t csl genv) ★ (SchI.t).
 
   Local Definition SchInSpc : spc_incl (SchAS.spc u spc_user_s) spc_s.
   Proof.
-    ii; rewrite /spc_s /SchAS.spc /MemA.spc /IncrMainAS.spc; unseal CRIS; split; [prove_nodup|ii].
+    ii; rewrite /spc_s /SchAS.spc /MemA.spc /IncrAS.spc; unseal CRIS; split; [prove_nodup|ii].
     ss; des_ifs; rewrite ->eq_rel_dec_correct in *; des_ifs.
   Qed.
-  Local Definition MainInSpc : spc_incl (IncrMainAS.spc u) spc_user_s.
+  Local Definition MainInSpc : spc_incl (IncrAS.spc u) spc_user_s.
   Proof.
-    ii; rewrite /spc_s /SchAS.spc /MemA.spc /IncrMainAS.spc; unseal CRIS; split; [prove_nodup|ii].
+    ii; rewrite /spc_s /SchAS.spc /MemA.spc /IncrAS.spc; unseal CRIS; split; [prove_nodup|ii].
     ss; des_ifs; rewrite ->eq_rel_dec_correct in *; des_ifs.
   Qed.
   Local Definition MemInSpc : spc_incl MemA.spc spc_s.
   Proof.
-    ii; rewrite /spc_s /SchAS.spc /MemA.spc /IncrMainAS.spc; unseal CRIS; split; [prove_nodup|ii].
+    ii; rewrite /spc_s /SchAS.spc /MemA.spc /IncrAS.spc; unseal CRIS; split; [prove_nodup|ii].
     ss; des_ifs; rewrite ->eq_rel_dec_correct in *; des_ifs.
   Qed.
 
   Local Definition init_cond : iProp Σ := MemA.init_cond csl genv ∗ SchA.init_cond.
-  Local Definition main_fsp : fspec := IncrMainAS.main_spec u.
+  Local Definition main_fsp : fspec := IncrAS.main_spec u.
 
   (* Apply cancellation to linked spec module *)
   Lemma cancel_src :
@@ -65,7 +65,9 @@ Module IncrAll.
   (* Refinement between spec/impl of whole program (linked module) *)
   Lemma src_tgt : refines (mod_src, init_cond) (mod_tgt, emp%I).
   Proof.
-    hexploit (IncrIA.ctxr u spc_s spc_user_s spc_s); eauto using SchInSpc, MainInSpc, MemInSpc.
+    hexploit (IncrIA.ctxr u 0 spc_s (to_spc (SchAS.spc 0 (to_spc []))) spc_user_s spc_s).
+    all: eauto using SchInSpc, MainInSpc, MemInSpc.
+    { rewrite /SchAS.spc; unseal CRIS. split; ii; ss. prove_nodup. }
     i; eapply ctxr_refines.
     rewrite -[(mod_src, _)]hmod_addc_empty_l.
     rewrite -[(mod_tgt, _)]hmod_addc_empty_r.
@@ -74,14 +76,19 @@ Module IncrAll.
     rewrite assoc. eapply ctxr_compose_hor.
     { etrans.
       { eapply ctxr_cond_frameR.
-        replace (SMod.to_hmod _ _ (IncrMainA.Mod u)) with (IncrMainA.t u spc_s); cycle 1.
-        { rewrite /IncrMainA.t; unseal CRIS; ss. }
+        replace (SMod.to_hmod _ _ (IncrA.Mod u)) with (IncrA.t u spc_s); cycle 1.
+        { rewrite /IncrA.t; unseal CRIS; ss. }
         replace (SMod.to_hmod _ _ MemA.Mod) with (MemA.t u spc_s); cycle 1.
         { rewrite /MemA.t; unseal CRIS; ss. }
         eauto.
       }
-      { eapply ctxr_frameL. etrans; first eapply ctxr_cond_frameL, MemIA.ctxr.
-        { eauto using MemInSpc. }
+      { rewrite ?hmod_add_assoc. eapply ctxr_frameL.
+        etrans.
+        { eapply ctxr_cond_frameR. eapply main_adequacy, FaaIA.sim. instantiate (1:=to_spc []).
+          rewrite /SchAS.spc; unseal CRIS. split; ii; ss. prove_nodup.
+        }
+        etrans.
+        { eapply ctxr_cond_frameL, ctxr_frameL, MemIA.ctxr. eauto using MemInSpc. }
         { eapply ctxr_cond_strengthen; eauto. }
       }
     }
@@ -91,7 +98,7 @@ Module IncrAll.
     replace (SMod.to_hmod _ _ (SchA_link.Mod _)) with (SchA_link.t u spc_s); cycle 1.
     { unfold_hmod; ss. }
     eapply SchIA.sim; eauto using SchInSpc.
-    { rewrite /spc_sub /spc_user_s /spc_s /IncrMainAS.spc /MemA.spc; unseal CRIS. ii; ss.
+    { rewrite /spc_sub /spc_user_s /spc_s /IncrAS.spc /MemA.spc; unseal CRIS. ii; ss.
       des_ifs; rewrite ->eq_rel_dec_correct in *; des_ifs.
     }
   Qed.
@@ -112,7 +119,7 @@ Module IncrAll.
   Proof.
     move: (cancel_tgt)=>H; rewrite /refines in H; ss.
     hexploit H.
-    { rewrite /mod_tgt /IncrMainI.t /MemI.t /SchI.t; unseal CRIS; prove_nodup. }
+    { rewrite /mod_tgt /IncrI.t /MemI.t /SchI.t /FaaI.t; unseal CRIS; prove_nodup. }
     clear H; intros [WF H].
     destruct (H (IRΣ ⋅ initial_resource_own_admin)).
     { apply IRΣ_valid. }
