incr/IncrMainHeader.v
@@ -1,6 +1,0 @@
-Require Import CRIS.
-
-Module MainHdr.
-  Definition main := "CRIS_init".
-  Definition f := "f".
-End MainHdr.
