incr/IncrA.v
@@ -1,0 +1,127 @@
+Require Import CRIS.
+Require Export ImpPrelude IncrHeader SchHeader SchA SchTactics MemHeader MemA.
+From iris Require Import frac_auth numbers.
+
+Class IncrAGΓ (Γ : HRA) := {
+  #[local] RA_inG :: inG (frac_authR ZR) Γ;
+}.
+Definition IncrAΓ : HRA := #[frac_authR ZR].
+Global Instance subG_GΓ {Γ : HRA} : subG IncrAΓ Γ → IncrAGΓ Γ.
+Proof. solve_inG. Defined.
+Hint Unfold subG_GΓ IncrAΓ : GRA_index.
+
+Module FaaA. Section FaaA.
+  Context `{!invG α Σ Γ, !subG Γ Σ, !sinvG Σ Γ α β τ, !memGΓ Γ}.
+  Context `{!SchAGΣ Σ, !SchAGΓ Γ}.
+
+  Definition faa_spec u : fspec :=
+    w_fspec_sch u (fspec_simple (λ '(b, ofs), (λ arg, ⌜arg = [Vptr b ofs]↑⌝, λ ret, ⌜ret = tt↑⌝)))%I.
+
+  Definition spc u : alist string fspec :=
+    [(FaaHdr.faa, faa_spec u)].
+
+  Definition scopes : list string := [].
+
+  Definition faa : list val → itree hmodE unit :=
+    λ arg,
+      '(b, ofs) : mblock * ptrofs <- (pargs [Tptr] arg)?;;
+      𝒴;;;
+        'v : Z <- trigger (Take Z);;
+        trigger (Assume ((b, ofs) ↦ Vint v));;;
+        trigger (Guarantee ((b, ofs) ↦ Vint (v + 1)));;;
+      𝒴;;; Ret tt.
+
+  Definition fnsems u := [(FaaHdr.faa, (scopes, mk_specbody (faa_spec u) (cfunN faa)))].
+
+  Program Definition Mod u : SMod.t := {|
+    SMod.scopes := scopes;
+    SMod.fnsems := fnsems u;
+    SMod.initial_st := [];
+  |}.
+  Solve All Obligations with prove_scope.
+  Next Obligation. prove_nodup. Qed.
+
+  Definition t u spc : HMod.t := Seal.sealing CRIS (SMod.to_hmod (wsim_ginv u ⊤) spc (Mod u)).
+End FaaA. End FaaA.
+
+Module IncrAS. Section IncrAS.
+  Context `{!invG α Σ Γ, !subG Γ Σ, !sinvG Σ Γ α β τ}.
+  Context `{!SchAGΣ Σ, !SchAGΓ Γ, !memGΓ Γ, !IncrAGΓ Γ}.
+
+  Definition N_main : namespace := (nroot .@ IncrHdr.main).
+
+  Definition counter γ q (v : Z) : iProp Σ := own γ (◯F{q} v).
+  Definition counter_syn {n} γ q (v : Z) : GTerm.t n := <own> γ (◯F{q} v).
+  Definition counter_auth γ (v : Z) : iProp Σ := own γ (●F v).
+
+  Definition ccounter_syn n γ blk ofs : GTerm.t n :=
+    (∃ v : τ{Z, n},
+      <own> base_γ (mem_points_to_singleton_r (blk, ofs) 1%Qp (Vint v))
+      ∗ <own> γ (frac_auth_auth v))%SAT.
+
+  Definition incr_inv u n γ blk ofs : iProp Σ :=
+    inv u n N_main (ccounter_syn n γ blk ofs).
+
+  (* rules *)
+  Lemma counter_op γ v1 q1 v2 q2 :
+    counter γ q1 v1 ∗ counter γ q2 v2 ⊣⊢ counter γ (q1 + q2) (v1 ⋅ v2).
+  Proof. rewrite /counter -own_op -frac_auth_frag_op //. Qed.
+
+  Lemma counter_incr v' γ v1 q1 v2 :
+    counter γ q1 v1 ∗ counter_auth γ v2 ==∗ counter γ q1 (v1 + v') ∗ counter_auth γ (v2 + v').
+  Proof.
+    rewrite /counter /counter_auth -own_op. iIntros "C".
+    iMod (own_update with "C") as "[C CA]".
+    { rewrite comm. eapply frac_auth_update, (Z_local_update _ _ (v2 + v') (v1 + v')); lia. }
+    iFrame; done.
+  Qed.
+
+  Definition incr_spec u : fspec :=
+    w_fspec_sch u
+      (fspec_simple (λ '(blk, ofs, v, γ),
+        (λ varg, ⌜varg = ([Vptr blk ofs]↑↑)↑⌝ ∗ counter γ (1/2) v ∗ incr_inv u 0 γ blk ofs,
+        λ vret, ⌜vret = (tt↑↑)↑⌝ ∗ counter γ (1/2) (v + 2))
+      ))%I.
+
+  Definition main_spec u : fspec :=
+    w_fspec_sch u (fspec_simple (λ _ : unit, (λ arg, ⌜arg = tt↑⌝, λ ret, ⌜ret = tt↑⌝)))%I.
+
+  Definition spc u : alist string fspec :=
+    [(IncrHdr.incr, incr_spec u);
+     (IncrHdr.main, main_spec u)].
+End IncrAS. End IncrAS.
+
+Module IncrA. Section IncrA.
+  Context `{!invG α Σ Γ, !subG Γ Σ, !sinvG Σ Γ α β τ}.
+  Context `{!SchAGΣ Σ, !SchAGΓ Γ, !memGΓ Γ, !IncrAGΓ Γ}.
+
+  Definition scopes : list string := [].
+
+  Definition incr : list val → itree hmodE unit :=
+    λ _, 𝒴;;; Ret tt.
+
+  Definition main : unit → itree hmodE unit :=
+    λ _,
+      𝒴;;; 'ptr_raw : val <- ccallU MemHdr.alloc [Vint 1%Z];;
+      𝒴;;; tid1 <- Sch.spawn (IncrHdr.incr, [ptr_raw]↑↑);;
+      𝒴;;; tid2 <- Sch.spawn (IncrHdr.incr, [ptr_raw]↑↑);;
+      𝒴;;; Sch.join tid1;;;
+      𝒴;;; Sch.join tid2;;;
+      𝒴;;; trigger (IO (O:=unit) "OUT" 4%Z);;;
+      𝒴;;; Ret tt.
+
+  Definition fnsems u :=
+    [(IncrHdr.incr, (scopes, mk_specbody (IncrAS.incr_spec u) (cfunN (sfunN incr))));
+     (IncrHdr.main, (scopes, mk_specbody (IncrAS.main_spec u) (cfunN main)))].
+
+  Program Definition Mod u : SMod.t := {|
+    SMod.scopes := scopes;
+    SMod.fnsems := fnsems u;
+    SMod.initial_st := [];
+  |}.
+  Solve All Obligations with prove_scope.
+  Next Obligation. prove_nodup. Qed.
+
+  Definition t u spc : HMod.t :=
+    Seal.sealing CRIS (SMod.to_hmod (wsim_ginv u ⊤) spc (Mod u)).
+End IncrA. End IncrA.
