incr/IncrHeader.v
@@ -1,0 +1,10 @@
+Require Import CRIS.
+
+Module FaaHdr.
+  Definition faa := "faa".
+End FaaHdr.
+
+Module IncrHdr.
+  Definition main := "CRIS_init".
+  Definition incr := "incr".
+End IncrHdr.
