incr/IncrI.v
@@ -1,0 +1,65 @@
+Require Import CRIS.
+Require Import ImpPrelude IncrHeader MemHeader SchHeader.
+
+Module FaaI. Section FaaI.
+  Context {Σ : GRA}.
+
+  Definition scopes : list string := [].
+
+  Definition faa : list val → itree pmodE unit :=
+    λ arg,
+      𝒴;;; '_ : val <- MemHdr.faa arg;;
+      𝒴;;; Ret tt.
+
+  Definition fnsems := [(FaaHdr.faa, (scopes, cfunU faa))].
+
+  Program Definition Mod : PMod.t := {|
+    PMod.scopes := scopes;
+    PMod.fnsems := fnsems;
+    PMod.initial_st := [];
+  |}.
+  Solve All Obligations with prove_scope.
+  Next Obligation. prove_nodup. Qed.
+
+  Definition t : HMod.t := Seal.sealing CRIS (PMod.to_hmod Mod).
+End FaaI. End FaaI.
+
+Module IncrI. Section IncrI.
+  Context {Σ : GRA}.
+
+  Definition scopes : list string := [].
+
+  Definition incr : list val → itree pmodE unit :=
+    λ arg,
+      𝒴;;; '_ : unit <- ccallU FaaHdr.faa arg;;
+      𝒴;;; '_ : unit <- ccallU FaaHdr.faa arg;;
+      𝒴;;; Ret tt.
+
+  Definition main : unit → itree pmodE unit :=
+    λ _,
+      𝒴;;; 'ptr_raw : val <- ccallU MemHdr.alloc [Vint 1%Z];;
+      𝒴;;; '(blk, ofs) : mblock * ptrofs <- (pargs [Tptr] [ptr_raw])?;;
+      𝒴;;; '_ : val <- ccallU MemHdr.store [Vptr blk ofs; Vint 0%Z];;
+      𝒴;;; tid1 <- Sch.spawn (IncrHdr.incr, [Vptr blk ofs]↑↑);;
+      𝒴;;; tid2 <- Sch.spawn (IncrHdr.incr, [Vptr blk ofs]↑↑);;
+      𝒴;;; Sch.join tid1;;;
+      𝒴;;; Sch.join tid2;;;
+      𝒴;;; 'v_raw : val <- ccallU MemHdr.load [Vptr blk ofs];;
+      𝒴;;; 'v : Z <- (pargs [Tint] [v_raw])?;;
+      𝒴;;; '_ : unit <- trigger (IO "OUT" v);;
+      𝒴;;; Ret tt.
+
+  Definition fnsems :=
+    [(IncrHdr.incr, (scopes, cfunU (sfunU incr)));
+     (IncrHdr.main, (scopes, cfunU main))].
+
+  Program Definition Mod : PMod.t := {|
+    PMod.scopes := scopes;
+    PMod.fnsems := fnsems;
+    PMod.initial_st := [];
+  |}.
+  Solve All Obligations with prove_scope.
+  Next Obligation. prove_nodup. Qed.
+
+  Definition t : HMod.t := Seal.sealing CRIS (PMod.to_hmod Mod).
+End IncrI. End IncrI.
