incr/IncrIAproof.v
@@ -1,0 +1,322 @@
+Require Import CRIS.
+Require Import IncrI IncrA SchA MemA SchTactics.
+From iris Require Import frac_auth numbers.
+
+Module FaaIA. Section FaaIA.
+  Context `{!invG α Σ Γ, !subG Γ Σ, !sinvG Σ Γ α β τ}.
+  Context `{!SchAGΣ Σ, !SchAGΓ Γ, !memGΓ Γ}.
+  Context (u_s u_mem : univ_id).
+  Context (spc_s spc_mem spc_user_s : string → option fspec).
+  Context (SchInSpc : spc_incl (SchAS.spc u_s spc_user_s) spc_s).
+
+  Definition Ist : nat → alist key Any.t → alist key Any.t → iProp Σ := λ _ _ _, emp%I.
+
+  Local Definition MemA := (MemA.t u_mem spc_mem).
+  Local Definition FaaA := (FaaA.t u_s spc_s).
+  Local Definition FaaI := (FaaI.t).
+  Local Definition IstFull := (IstProd (IstSB FaaA.(HMod.scopes) Ist) IstEq).
+  Local Definition MA := (FaaA ★ MemA).
+  Local Definition MI := (FaaI ★ MemA).
+
+  Lemma faa_simF : HSim.sim_fun open MA MI IstFull FaaHdr.faa.
+  Proof.
+    init_simF u_s 0.
+    steps_l. iDestruct "ASM" as "[TID [-> ->]]". hss. rename q3 into b, q4 into ofs, q1 into tid.
+    steps_l. steps_r.
+
+    (* tgt yield *)
+    sch_yield_r.
+    iFrame. clear nths st_src st_tgt NODD NODS. iIntros (nths st_s st_t NODS NODD) "IST TID".
+    (* src yield *)
+    sch_yield_l.
+    (* src take pointsto *)
+    steps_l. rename q into v.
+    (* tgt inline - load *)
+    rewrite /MemHdr.faa. inline_r.
+    (* tgt prove preconditions for load *)
+    force_r (b, ofs, Vint v, 1%Qp). forces_r. iFrame. iSplit; first eauto.
+    (* tgt get postconditions from load *)
+    steps_r. iDestruct "GRT" as "[[PT ->] ->]". hss. steps_r.
+    (* tgt inline - store *)
+    inline_r. force_r (b, ofs, Vint (v + 1)). forces_r. iFrame. iSplit; first eauto.
+    (* tgt get postconditions from store *)
+    steps_r. iDestruct "GRT" as "[[PT ->] ->]". hss. steps_r.
+    (* src give pointsto *)
+    force_l. iFrame. steps_l.
+    (* tgt yield *)
+    sch_yield_r.
+    iFrame. clear nths st_s st_t NODD NODS. iIntros (nths st_s st_t NODS NODD) "IST TID".
+    (* tgt terminate *)
+    steps_r.
+    (* src yield & terminate *)
+    sch_yield_l. steps_l. forces_l. iFrame. iSplit; eauto. steps_l. step. iFrame. done.
+  (*FAST*)Qed.
+
+  Lemma sim : HSim.t open MA MI emp%I IstFull.
+  Proof.
+    init_sim.
+    { iIntros "_"; iExists [], [], [], []; eauto. }
+    { eapply faa_simF. }
+  Qed.
+End FaaIA. End FaaIA.
+
+Module IncrIA. Section IncrIA.
+  Import IncrAS.
+  Context `{!invG α Σ Γ, !subG Γ Σ, !sinvG Σ Γ α β τ}.
+  Context `{!SchAGΣ Σ, !SchAGΓ Γ, !memGΓ Γ, !IncrAGΓ Γ}.
+
+  Definition Ist : nat → alist key Any.t → alist key Any.t → iProp Σ := λ _ _ _, emp%I.
+
+  Context (u_s u_t : univ_id).
+  Context `{u_s > u_t}.
+  Context (spc_s spc_t spc_user_s spc_mem : string → option fspec).
+  Context (SchInSpcS : spc_incl (SchAS.spc u_s spc_user_s) spc_s).
+  Context (MemInSpc : spc_incl MemA.spc spc_s).
+  Context (MainInSpc : spc_incl (IncrAS.spc u_s) spc_user_s).
+  Context (SchInSpcT : spc_incl (SchAS.spc u_t (to_spc [])) spc_t).
+
+  Local Definition MemA := (MemA.t u_s spc_mem).
+  Local Definition IncrA := (IncrA.t u_s spc_s).
+  Local Definition IncrI := (IncrI.t).
+  Local Definition IstFull := (IstProd (IstSB IncrA.(HMod.scopes) Ist) IstEq).
+  Local Definition MA := (IncrA ★ MemA).
+  Local Definition MI := ((IncrI ★ FaaA.t u_t spc_t) ★ MemA).
+
+  Lemma f_spawnable γ v blk ofs :
+    SchAS.fspec_spawnable u_s (IncrAS.incr_spec u_s)
+      (λ varg arg,
+        ⌜varg = arg ∧ varg = ([Vptr blk ofs]↑↑)⌝
+        ∗ counter γ (1/2) v
+        ∗ incr_inv u_s 0 γ blk ofs)%I
+      (λ vret ret,
+        existT 0 ((⌜vret = ret ∧ vret = tt↑↑⌝ ∗ counter_syn γ (1/2) (v + 2))%SAT)).
+  Proof.
+    rewrite /SchAS.fspec_spawnable /w_fspec /fspec_virtual /precond /postcond /incr_spec /=.
+    ii; ss. eexists (x_src, (blk, ofs, v, γ)); split; red; ii.
+    - rewrite /precond /w_fspec_sch /fspec_simple /w_fspec /precond /=.
+      iIntros "[W [% [-> [TID [% [-> [[-> ->] [C #INV]]]]]]]]". iFrame. eauto.
+    - rewrite /postcond /w_fspec_sch /fspec_simple /w_fspec /postcond /=.
+      iIntros "[W [TID [[-> C] ->]]]". iFrame. iExists _; iSplitR; eauto.
+      iExists _; iSplitR; eauto. SL_red. iSplitR; eauto.
+  Qed.
+
+  Lemma incr_simF : HSim.sim_fun open MA MI IstFull IncrHdr.incr.
+  Proof.
+    init_simF u_s u_t.
+
+    steps_l. iDestruct "ASM" as "[TID [[-> [C #INV]] ->]]". hss.
+    rename q7 into b, q8 into ofs. rename q4 into γ, q6 into v. rename q1 into tid.
+
+    steps_l. hss. steps_l.
+    steps_r. hss. steps_r.
+    rewrite /IncrI.incr /IncrA.incr /=. steps_r.
+
+    sch_yield_r.
+    iSplitL "IST"; iFrame.
+    clear nths NODS NODD. iIntros (nths st_s st_t NODS NODD) "IST TID".
+
+    (* tgt inline - faa *)
+    inline_r. hss. steps_r. force_r (tid, (b, ofs)). forces_r. iFrame. iSplit; eauto. steps_r. hss.
+    steps_r.
+
+    sch_yield_r.
+    iSplitL "IST"; iFrame.
+    clear nths st_s st_t NODS NODD. iIntros (nths st_s st_t NODS NODD) "IST".
+
+    rewrite /IncrAS.incr_inv.
+    iInv "INV" as "I" "IA". SL_red.
+    iDestruct "I" as (x) "PT". SL_red. iDestruct "PT" as "[PT CA]".
+
+    (* operational atomicity here *)
+    force_r x. steps_r. force_r. iFrame. steps_r.
+
+    iMod (counter_incr 1 with "[C CA]") as "[C CA]"; first iFrame.
+    iMod ("IA" with "[GRT CA]") as "_".
+    { iExists (x + 1)%Z; SL_red; ss; iFrame. }
+
+    sch_yield_r. iFrame.
+    clear nths st_s st_t NODS NODD. iIntros (nths st_s st_t NODS NODD) "IST".
+
+    steps_r. iDestruct "GRT" as "[TID [-> _]]". hss. steps_r.
+
+    sch_yield_r. iFrame.
+    clear nths st_s st_t NODS NODD. iIntros (nths st_s st_t NODS NODD) "IST TID".
+    (* tgt inline - faa *)
+    inline_r. hss. steps_r. force_r (tid, (b, ofs)). forces_r. iFrame. iSplit; eauto. steps_r. hss.
+    steps_r.
+
+    sch_yield_r.
+    iSplitL "IST"; iFrame.
+    clear nths st_s st_t NODS NODD. iIntros (nths st_s st_t NODS NODD) "IST".
+
+    rewrite /IncrAS.incr_inv.
+    iInv "INV" as "I" "IA". SL_red.
+    clear x. iDestruct "I" as (x) "PT". SL_red. iDestruct "PT" as "[PT CA]".
+
+    (* operational atomicity here *)
+    force_r x. steps_r. force_r. iFrame. steps_r.
+
+    iMod (counter_incr 1 with "[C CA]") as "[C CA]"; first iFrame.
+    iMod ("IA" with "[GRT CA]") as "_".
+    { iExists (x + 1)%Z; SL_red; ss; iFrame. }
+
+    sch_yield_r. iFrame.
+    clear nths st_s st_t NODS NODD. iIntros (nths st_s st_t NODS NODD) "IST".
+
+    steps_r. iDestruct "GRT" as "[TID [-> _]]". hss. steps_r.
+
+    sch_yield_r. iFrame.
+    clear nths st_s st_t NODS NODD. iIntros (nths st_s st_t NODS NODD) "IST TID".
+
+    steps_r.
+    sch_yield_l.
+    steps_l. force_l. steps_l. force_l.
+    iSplitL "TID C".
+    { iFrame. replace (v + 1 + 1)%Z with (v + 2)%Z by lia. iFrame. eauto. }
+    steps_l. step; eauto.
+  (*FAST*)Qed.
+
+  Lemma main_simF : HSim.sim_fun open MA MI IstFull IncrHdr.main.
+  Proof.
+    init_simF u_s u_t.
+
+    steps_l. iDestruct "ASM" as "[TID [-> ->]]". hss.
+    steps_l.
+
+    (* src/tgt yield *)
+    steps_r.
+    sch_yield_r. iFrame.
+    clear nths NODS NODD. iIntros (nths st_s st_t NODS NODD) "IST TID".
+
+    sch_yield_l.
+
+    (* src/tgt alloc *)
+    steps_l. force_l 1. steps_l. force_l. steps_l.
+    force_l. iSplit; eauto. steps_l.
+    steps_r. call "IST".
+    steps_l. iDestruct "ASM" as "[[%b [-> [PT _]]] ->]". hss.
+    steps_r. hss. steps_r.
+
+    (* tgt yield *)
+    sch_yield_r. iFrame.
+    clear nths st_s st_t NODS NODD. iIntros (nths st_s st_t NODS NODD) "IST TID".
+    steps_r.
+    sch_yield_r. iFrame.
+    clear nths st_s st_t NODS NODD. iIntros (nths st_s st_t NODS NODD) "IST TID".
+
+    (* tgt store *)
+    inline_r. steps_r. force_r (b, 0%Z, Vint 0%Z). steps_r.
+    force_r. steps_r. force_r. iSplitL "PT".
+    { iFrame. eauto. }
+    steps_r. iDestruct "GRT" as "[[PT ->] ->]". hss. steps_r.
+
+    (* src/tgt yield *)
+    sch_yield_r. iFrame.
+    clear nths st_s st_t NODS NODD. iIntros (nths st_s st_t NODS NODD) "IST TID".
+    sch_yield_l.
+
+    iApply (wsim_own_alloc (●F 0%Z ⋅ ◯F{1} 0%Z)).
+    { apply frac_auth_valid; ss. }
+
+    iIntros "[%γc [A F]]".
+    iMod (inv_alloc (ccounter_syn 0 γc b 0%Z) _ _ _ N_main with "[PT A]") as "#I"; eauto.
+    { rewrite /ccounter_syn; SL_red; iExists 0; SL_red; iFrame. }
+    iPoseProof (counter_op with "[F]") as "[F1 F2]".
+    { rewrite -Qp.half_half -{2}(Z.add_0_r 0%Z). iApply "F". }
+
+    iCombine "F1 I" as "F1". iCombine "F2 I" as "F2".
+    steps_l. steps_r.
+
+    (* src/tgt spawns *)
+    sch_spawn; eauto using f_spawnable.
+    { eapply MainInSpc. ss. }
+    iFrame. iSplitL "" ; eauto.
+    clear nths st_s st_t NODS NODD. iIntros (tid nths st_s st_t NODS NODD) "IST TID TKN".
+
+    (* src/tgt yield *)
+    sch_yield_r. iFrame.
+    clear nths st_s st_t NODS NODD. iIntros (nths st_s st_t NODS NODD) "IST TID".
+
+    sch_yield_l.
+
+    sch_spawn; eauto using f_spawnable.
+    { eapply MainInSpc. ss. }
+    iFrame. iSplitL "" ; eauto.
+    clear nths st_s st_t NODS NODD. iIntros (tid2 nths st_s st_t NODS NODD) "IST TID TKN2".
+
+    (* src/tgt yield *)
+    sch_yield_r. iFrame.
+    clear nths st_s st_t NODS NODD. iIntros (nths st_s st_t NODS NODD) "IST TID".
+
+    sch_yield_l.
+
+    sch_join. iFrame.
+    clear nths st_s st_t NODS NODD. iIntros (nths st_s st_t ? ? NODS NODD) "IST TID Q /=". SL_red.
+    iDestruct "Q" as "[[-> ->] Q]".
+
+    sch_yield_r. iFrame.
+    clear nths st_s st_t NODS NODD. iIntros (nths st_s st_t NODS NODD) "IST TID".
+
+    sch_yield_l.
+
+    sch_join. iFrame.
+    clear nths st_s st_t NODS NODD. iIntros (nths st_s st_t ? ? NODS NODD) "IST TID Q2 /="; SL_red.
+    iDestruct "Q2" as "[[-> ->] Q2]".
+
+    sch_yield_r. iFrame.
+    clear nths st_s st_t NODS NODD. iIntros (nths st_s st_t NODS NODD) "IST TID".
+
+    iInv "I" as "INV" "INVA"; iEval (SL_red) in "INV"; iDestruct "INV" as "[%x INV]".
+    iEval (SL_red) in "INV". iDestruct "INV" as "[PT C]".
+    iCombine "C Q Q2" as "C" gives %[_ WF%frac_auth_agree]. inv WF; ss.
+    iDestruct "C" as "[CA CF]".
+
+    inline_r. steps_r. force_r (b, 0%Z, (Vint 4), 1%Qp). steps_r. forces_r.
+    iSplitL "PT"; eauto.
+    steps_r. iDestruct "GRT" as "[[PT ->] ->]". hss. steps_r.
+
+    iMod ("INVA" with "[CA PT]") as "_".
+    { SL_red. iExists 4; SL_red; iFrame. }
+
+    sch_yield_r. iFrame.
+    clear nths st_s st_t NODS NODD. iIntros (nths st_s st_t NODS NODD) "IST TID".
+
+    sch_yield_r. iFrame.
+    clear nths st_s st_t NODS NODD. iIntros (nths st_s st_t NODS NODD) "IST TID".
+
+    sch_yield_l. step.
+    steps_l. steps_r.
+
+    sch_yield_r. iFrame.
+    clear nths st_s st_t NODS NODD. iIntros (nths st_s st_t NODS NODD) "IST TID".
+    
+    sch_yield_l.
+    steps_l. force_l. steps_l. force_l. iSplitL "TID"; eauto.
+    steps_l. steps_r.
+    step. eauto.
+  (*FAST*)Qed.
+
+  Lemma sim : HSim.t open MA MI emp%I IstFull.
+  Proof.
+    init_sim.
+    { iIntros "_"; iExists [], [], [], []; eauto. }
+    { eapply incr_simF. }
+    { eapply main_simF. }
+  Qed.
+End IncrIA.
+
+Section ctxr.
+  Context `{!invG α Σ Γ, !subG Γ Σ, !sinvG Σ Γ α β τ}.
+  Context `{!SchAGΣ Σ, !SchAGΓ Γ, !memGΓ Γ, !IncrAGΓ Γ}.
+
+  Definition ctxr (u_s u_t : univ_id) (spc_s spc_t spc_user_s spc_mem : string → option fspec)
+      (SchInSpcS : spc_incl (SchAS.spc u_s spc_user_s) spc_s)
+      (SchInSpcT : spc_incl (SchAS.spc u_t (to_spc [])) spc_t)
+      (MainInSpc : spc_incl (IncrAS.spc u_s) spc_user_s)
+      (MemInSpc : spc_incl MemA.spc spc_s)
+      (Univ : u_s > u_t) :
+    ctx_refines
+      ((IncrA.t u_s spc_s)            ★ (MemA.t u_s spc_mem), emp%I)
+      ((IncrI.t ★ FaaA.t u_t spc_t)   ★ (MemA.t u_s spc_mem), emp%I).
+  Proof. eapply main_adequacy, sim; try solve_sch_spc; eauto. Qed.
+End ctxr. End IncrIA.
